%% LyX 2.1.3 created this file.  For more info, see http://www.lyx.org/.
%% Do not edit unless you really know what you are doing.
\documentclass[english]{article}
\usepackage[T1]{fontenc}
\usepackage[latin9]{inputenc}
\usepackage{geometry}
\geometry{verbose,tmargin=3cm,bmargin=3cm,lmargin=3cm,rmargin=3cm}
\usepackage{esint}
\usepackage{babel}
\begin{document}

\subsubsection*{CV Proof: Mitchell's Thrm}

Consider the CV problem with 
\[
\hat{\lambda}=\arg\min_{\lambda}\sum_{k=1}^{K}\|y-\hat{g}_{\lambda}(\cdot|D_{-k})\|_{k}^{2}
\]


We consider the behavior of 
\[
\hat{g}_{MCV}=\sum_{k=1}^{K}\hat{g}_{\lambda}(\cdot|D_{-k})
\]


and its generalization error 
\[
E_{D}\|\hat{g}_{MCV}(\cdot|D)-g^{*}\|^{2}=E_{D}\left[\int\left(\hat{g}_{MCV}(x|D)-g^{*}(x)\right)^{2}d\mu(x)\right]
\]


We will assume that $\sup_{g\in\mathcal{G}}\|g\|_{\infty}\le G$,
so Assumption A.1 and A.2 are satisfied.

Suppose the errors are bounded ($\|\epsilon\|_{\infty}<\infty$ ).

Suppose we can show 
\[
\|g_{\lambda_{1}}-g_{\lambda_{2}}\|_{\infty}\le\left|\lambda_{1}-\lambda_{2}\right|n^{\kappa}C
\]


So we get that
\[
E\left[\|g^{*}-\frac{1}{k}\sum_{k=1}^{K}g_{\hat{\lambda}}(\cdot|D_{-k})\|^{2}\right]\le(1+a)E\left[\|g^{*}-\frac{1}{k}\sum_{k=1}^{K}g_{\tilde{\lambda}}(\cdot|D_{-k})\|^{2}\right]+c_{a}J^{2}\max_{k=1:K}\frac{\left(\log n\right)^{2}}{n_{k}}
\]



\subsubsection*{Proof}

First note that the assumption A.2 is satisfied: 
\begin{eqnarray*}
\int\left(g^{*}(x)-g_{\lambda}(x|D_{0})\right)^{4}d\mu(x) & \le & \|\left(g^{*}-g_{\lambda}\right)^{2}\|_{1}\|\left(g^{*}-g_{\lambda}\right)^{2}\|_{\infty}\\
 & \le & 4G^{2}\|g^{*}-g_{\lambda}\|_{2}^{2}
\end{eqnarray*}


Let 
\[
\mathcal{Q}(T)=\left\{ q_{\lambda}(x,y)=(g^{*}-\hat{g}_{\lambda})^{2}:\lambda\in\Lambda\right\} 
\]


To compute the upper bound, we need the $\|\cdot\|_{\psi_{1}}$ and
$\|\cdot\|_{L_{2}}$ entropy of the function class 

\[
\mathcal{Q}_{d}^{L_{2}}(T)=\left\{ q\in\mathcal{Q}(T):\|Q(Z)\|_{2}\le\sqrt{d}\right\} 
\]


From our assumptions, we note that 
\begin{eqnarray*}
\|q_{\lambda_{1}}-q_{\lambda_{2}}\|_{\psi_{1}} & = & \|(g^{*}-g_{\lambda_{1}})^{2}-(g^{*}-g_{\lambda_{2}})^{2}\|_{\psi_{1}}\\
 & = & \|(g_{\lambda_{1}}-g_{\lambda_{2}})(2g^{*}-g_{\lambda_{1}}-g_{\lambda_{2}})\|_{\psi_{1}}\\
 & \le & \|g_{\lambda_{1}}-g_{\lambda_{2}}\|_{\infty}\|2g^{*}-g_{\lambda_{1}}-g_{\lambda_{2}}\|_{\infty}\\
 & \le & \left|\lambda_{1}-\lambda_{2}\right|4Cn^{\kappa}G
\end{eqnarray*}


and similarly for $\|\cdot\|_{L_{2}}$ (we're using a loose bound
for $\|\cdot\|_{L_{2}}$ since calculating its inverse/convex conjugate
is difficult).

Hence (for a different constant $\kappa$)

\[
H(u,\mathcal{Q}_{d}^{L_{2}}(T),\|\cdot\|_{\psi_{1}})\le J\left(\log\frac{1}{u}+\log(4Cn^{\kappa}G)\right)
\]


and

\[
H(u,\mathcal{Q}_{d}^{L_{2}}(T),\|\cdot\|_{L_{2}})\le J\left(\log\frac{1}{u}+\log(4Cn^{\kappa}G)\right)
\]


We calculate each component of the complexity term $J(d)$: 
\begin{eqnarray*}
\gamma_{1}(\mathcal{Q}_{d}^{L_{2}}(T),\|\cdot\|_{\psi_{1}}) & = & \int_{0}^{G}H(u,\mathcal{Q}_{d}^{L_{2}}(T),\|\cdot\|_{\psi_{1}})du\\
 & = & JG\left(1+\log(4Cn^{\kappa}G)\right)
\end{eqnarray*}


and

\begin{eqnarray*}
\gamma_{2}(\mathcal{Q}_{d}^{L_{2}}(T),\|\cdot\|_{L_{2}}) & = & \int_{0}^{\sqrt{d}}\left[H(u,\mathcal{Q}_{d}^{L_{2}}(T),\|\cdot\|_{L_{2}})\right]^{1/2}du\\
 & = & \sqrt{d}\int_{0}^{1}\left[J\left(\log\frac{1}{u}+\log(4Cn^{\kappa}G)\right)\right]^{1/2}du\\
 & \le & \sqrt{d}\left[\int_{0}^{1}J\left(\log\frac{1}{u}+\log(4Cn^{\kappa}G)\right)du\right]^{1/2}\\
 & = & \sqrt{d}\left[J\left(1+\log(4Cn^{\kappa}G)\right)\right]^{1/2}
\end{eqnarray*}


So we can define 
\begin{eqnarray*}
J(d) & \equiv & J\left(1+\log(4Cn^{\kappa}G)\right)\left[\sqrt{d}+\left(\max_{k=1:K}\frac{\log n_{k}}{\sqrt{n_{k}}}\right)\right]\\
 & \ge & \sqrt{d}\left[J\left(1+\log(4Cn^{\kappa}G)\right)\right]^{1/2}+\left(\max_{k=1:K}\frac{\log n_{k}}{\sqrt{n_{k}}}\right)JG\left(1+\log(4Cn^{\kappa}G)\right)
\end{eqnarray*}
 

Then$J^{-1}(b)$ is
\[
J^{-1}(b)=\left(\frac{b}{J\left(1+\log(4Cn^{\kappa}G)\right)}-\left(\max_{k=1:K}\frac{\log n_{k}}{\sqrt{n_{k}}}\right)\right)^{2}
\]


The convex conjugate of $J^{-1}(b)$ is
\[
\psi(v)=\frac{1}{2}\left(vJ\left(1+\log(4Cn^{\kappa}G)\right)\right)^{2}+J\left(1+\log(4Cn^{\kappa}G)\right)\left(\max_{k=1:K}\frac{\log n_{k}}{\sqrt{n_{k}}}\right)v
\]


Therefore
\begin{eqnarray*}
\epsilon_{q}(1/q) & = & \psi\left(\max_{k=1:K}\frac{2q(1+a)}{a\sqrt{n_{k}}}\right)\\
 & = & \frac{1}{2}\left(\frac{2q(1+a)}{a\sqrt{n_{k}}}J\left(1+\log(4Cn^{\kappa}G)\right)\right)^{2}+J\left(1+\log(4Cn^{\kappa}G)\right)\left(\max_{k=1:K}\frac{\log n_{k}}{\sqrt{n_{k}}}\right)\frac{2q(1+a)}{a\sqrt{n_{k}}}\\
 & \le & \max_{k=1:K}\left(\frac{2q(1+a)}{a\sqrt{n_{k}}}J\left(1+\log(4Cn^{\kappa}G)\right)\right)^{2}
\end{eqnarray*}


Finally, we get
\[
E\left[\|g^{*}-\frac{1}{k}\sum_{k=1}^{K}g_{\hat{\lambda}}(\cdot|D_{-k})\|^{2}\right]\le(1+a)E\left[\|g^{*}-\frac{1}{k}\sum_{k=1}^{K}g_{\tilde{\lambda}}(\cdot|D_{-k})\|^{2}\right]+\frac{c(1+a)^{2}}{a}\frac{J^{2}\left(1+\log(4Cn^{\kappa}G)\right)^{2}}{\min_{k=1:K}n_{k}}
\]

\end{document}
