%% LyX 2.1.3 created this file.  For more info, see http://www.lyx.org/.
%% Do not edit unless you really know what you are doing.
\documentclass[english]{article}
\usepackage[T1]{fontenc}
\usepackage[latin9]{inputenc}
\usepackage{geometry}
\geometry{verbose,tmargin=3cm,bmargin=3cm,lmargin=3cm,rmargin=3cm}
\usepackage{amsmath}
\usepackage{babel}
\begin{document}

\subsection*{Lemma PSD\_Matrix\_Inverse}

Suppose $A$ is a PSD matrix and $D$ is a diagonal matrix with positive
entries. Then for any vector $x$, we have 
\[
\|D^{-1}x\|\ge\|(A+D)^{-1}x\|
\]



\subsubsection*{Proof}

Notation: For matrix $B$, define $B^{2}=BB$.

It suffices to show that for all $x$, 
\[
x^{T}\left(D^{-2}-(A+D)^{-2}\right)x\ge0
\]


That is, we are interested in showing that $D^{-2}-(A+D)^{-2}$ is
PSD. This can be shown by noting that

\[
(A+D)^{2}\succeq D^{2}\implies D^{-2}\succeq(A+D)^{-2}
\]



\subsection*{Lemma: Lipschitz Definition Equivalence}

The following two conditions are equivalent:
\begin{enumerate}
\item For all $u>0$ and any $\lambda^{(1)},\lambda^{(2)}$ that satisfy
\[
\|\lambda^{(1)}-\lambda^{(2)}\|\le Cu
\]

\end{enumerate}
then 
\[
\|\hat{g}(\cdot|\lambda^{(1)})-\hat{g}(\cdot|\lambda^{(2)})\|_{D}\le u
\]

\begin{enumerate}
\item $\hat{g}(\cdot|\lambda)$ is $1/C$-Lipschitz in $\lambda$: 
\[
\|\hat{g}(\cdot|\lambda^{(1)})-\hat{g}(\cdot|\lambda^{(2)})\|_{D}\le\frac{1}{C}\|\lambda^{(1)}-\lambda^{(2)}\|
\]

\end{enumerate}

\subsubsection*{Proof}

It is clear that Condition 2 implies Condition 1. 

To show Condition 1 implies Condition 2, suppose for any $\lambda^{(1)},\lambda^{(2)}$,
we have 
\[
\|\lambda^{(1)}-\lambda^{(2)}\|=d=C\frac{d}{C}
\]


Then 
\[
\|\hat{g}(\cdot|\lambda^{(1)})-\hat{g}(\cdot|\lambda^{(2)})\|_{D}\le\frac{d}{C}=\frac{1}{C}\|\lambda^{(1)}-\lambda^{(2)}\|
\]

\end{document}
